work on untyped reduction

Untyped/Red.lean
@@ -1,51 +1,292 @@
 import Untyped.Subst
 import Untyped.Term
 
-@[simp]
-def conv : Nat -> Nat -> Term -> Term -> Bool
-| _, _, #x, #y => x == y
-| g1 + 1, g2, (`λ t) `@ a1, f2 `@ a2 => conv g1 g2 (t β[a1]) (f2 `@ a2)
-| g1, g2 + 1, f1 `@ a1, (`λ t) `@ a2 => conv g1 g2 (f1 `@ a1) (t β[a2])
-| g1, g2, f1 `@ a1, f2 `@ a2 => conv g1 g2 f1 f2 && conv g1 g2 a1 a2
-| g1, g2, `λ t1, `λ t2 => conv g1 g2 t1 t2
-| _, _, _, _ => false
-
 inductive Red : Term -> Term -> Prop where
 | beta : Red ((`λ b) `@ t) (b β[t])
 | app_congr1 : Red a a' -> Red (f `@ a) (f `@ a')
 | app_congr2 : Red f f' -> Red (f `@ a) (f' `@ a)
 | lam_congr : Red t t' -> Red (`λ t) (`λ t')
 
-inductive RedStar : Nat -> Term -> Term -> Prop where
-| refl : RedStar 0 t t
-| step : Red x y -> RedStar n y z -> RedStar (n + 1) x z
+inductive SpineRed : Term -> Term -> Prop where
+| beta : SpineRed ((`λ b) `@ t) (b β[t])
+| app : SpineRed f f' -> SpineRed a a' -> SpineRed (f `@ a) (f' `@ a')
+| lam : SpineRed t t' -> SpineRed (`λ t) (`λ t')
 
-inductive RedConv : Nat -> Nat -> Term -> Term -> Prop where
-| var : RedConv g1 g2 #x #x
-| beta_le : RedConv g1 g2 (t β[a1]) (f2 `@ a2) -> RedConv (g1 + 1) g2 ((`λ t) `@ a1) (f2 `@ a2)
-| beta_ri : RedConv g1 g2 (f1 `@ a1) (t β[a2])  -> RedConv g1 (g2 + 1) (f1 `@ a1) ((`λ t) `@ a2)
-| app : RedConv g1 g2 f1 f2 -> RedConv g1 g2 a1 a2 -> RedConv g1 g2 (f1 `@ a1) (f2 `@ a2)
-| lam : RedConv g1 g2 t1 t2 -> RedConv g1 g2 (`λ t1) (`λ t2)
+inductive ParRed : Term -> Term -> Prop where
+| beta : ParRed b b' -> ParRed t t' -> ParRed ((`λ b) `@ t) (b' β[t'])
+| app : ParRed a a' -> ParRed f f' -> ParRed (f `@ a) (f' `@ a')
+| lam : ParRed t t' -> ParRed (`λ t) (`λ t')
+| var : ParRed #x #x
+
+inductive Star (R : Term -> Term -> Prop) : Nat -> Term -> Term -> Prop where
+| refl : Star R n t t
+| step : Star R n x y -> R y z -> Star R (n + 1) x z
+
+def Conv (R : Term -> Term -> Prop) (g1 g2 : Nat) (x y : Term) : Prop :=
+  ∃ z, Star R g1 x z ∧ Star R g2 y z
 
 infix:40 " -β> " => Red
-notation:39 x:39 " -β[" n:39 "]>* " y:39 => RedStar n x y
-notation:38 x:38 " =β[" g1:38 ";" g2:38 "]= " y:38 => RedConv g1 g2 x y
+infix:40 " =β> " => ParRed
+infix:40 " -s> " => SpineRed
+notation:39 x:39 " -β[" n:39 "]>* " y:39 => Star Red n x y
+notation:39 x:39 " =β[" n:39 "]>* " y:39 => Star ParRed n x y
+notation:39 x:39 " -s[" n:39 "]>* " y:39 => Star SpineRed n x y
+notation:38 x:38 " =β[" g1:38 ";" g2:38 "]= " y:38 => Conv Red g1 g2 x y
+notation:38 x:38 " ≡β[" g1:38 ";" g2:38 "]≡ " y:38 => Conv ParRed g1 g2 x y
+notation:38 x:38 " =s[" g1:38 ";" g2:38 "]= " y:38 => Conv SpineRed g1 g2 x y
 
-namespace RedConv
+namespace Star
+  @[simp]
+  def star (f : Term -> Term) : Nat -> Term -> Term
+  | 0, t => t
+  | n + 1, t => star f n (f t)
 
-  theorem weaken : RedConv g1 g2 x y -> RedConv (g1 + k1) (g2 + k2) x y := by sorry
+  theorem weaken k : Star R g x y -> Star R (g + k) x y := by
+  intro r; induction r generalizing k
+  case _ => constructor
+  case _ n _ _ _ _ r2 ih =>
+    have lem : n + 1 + k = n + k + 1 := by omega
+    rw [lem]; apply Star.step (ih k) r2
 
-  theorem conv_sound : conv g1 g2 x y -> x =β[g1;g2]= y := by
-  intro h; induction g1, g2, x, y using conv.induct <;> simp at *
-  case _ => subst h; constructor
-  case _ ih => apply beta_le; apply ih h
-  case _ ih _ => apply beta_ri; apply ih h
-  case _ ih1 ih2 _ _ => apply app (ih1 h.1) (ih2 h.2)
-  case _ ih => apply lam (ih h)
+  theorem trans : Star R g1 x y -> Star R g2 y z -> Star R (g1 + g2) x z := by
+  intro r1 r2; induction r2 generalizing g1 x
+  case _ n t => apply weaken n r1
+  case _ n a b c _ r2 ih => apply Star.step (ih r1) r2
 
-  theorem sym : x =β[g1;g2]= y -> y =β[g2;g1]= x := by sorry
+  theorem promote (Rprm : ∀ {x y}, R1 x y -> R2 x y) :
+    Star R1 n x y -> Star R2 n x y
+  := by
+  intro r; induction r
+  case _ => constructor
+  case _ _ r ih => constructor; apply ih; apply Rprm r
 
-  theorem trans : x =β[gx;gy1]= y -> y =β[gy2;gz]= z -> x =β[gx + gy2;yz + gy1]= z := by sorry
+  theorem star_sound n t : (∀ t, R t (f t)) -> Star R n t (star f n t) := by
+  intro h
+  have lem : ∀ {t n}, R (star f n t) (star f n (f t)) := by
+    intro t n; induction n generalizing t; simp; apply h _
+    case _ n ih => simp; apply ih
+  induction n
+  case _ => simp; constructor
+  case _ n ih =>
+    constructor; apply ih; simp; apply lem
+end Star
 
+namespace Conv
+  @[simp]
+  def conv (f : Term -> Term) (g1 g2 : Nat) (a b : Term) : Bool :=
+    Star.star f g1 a == Star.star f g2 b
 
-end RedConv
+  theorem weaken k1 k2 : Conv R g1 g2 x y -> Conv R (g1 + k1) (g2 + k2) x y := by
+  intro h; cases h; case _ w h =>
+    exists w; apply And.intro
+    apply Star.weaken k1 h.1; apply Star.weaken k2 h.2
+
+  theorem promote (Rprm : ∀ {x y}, R1 x y -> R2 x y) :
+    Conv R1 g1 g2 x y -> Conv R2 g1 g2 x y
+  := by
+  intro h; cases h; case _ w h =>
+    exists w; apply And.intro
+    apply Star.promote Rprm h.1; apply Star.promote Rprm h.2
+
+  theorem conv_sound : (∀ t, R t (f t)) -> conv f g1 g2 a b -> Conv R g1 g2 a b := by
+  intro h1 h2; simp at h2
+  replace h2 := @LawfulBEq.eq_of_beq Term _ _ _ _ h2
+  have lem1 := Star.star_sound g1 a h1
+  have lem2 := Star.star_sound g2 b h1
+  exists (Star.star f g1 a); apply And.intro
+  apply lem1; rw [h2]; apply lem2
+
+end Conv
+
+namespace ParRed
+  @[simp]
+  def pcompl : Term -> Term
+  | `λt `@  a => (pcompl t) β[pcompl a]
+  | f `@ a => (pcompl f) `@ (pcompl a)
+  | `λt => `λ(pcompl t)
+  | #x => #x
+
+  @[simp]
+  def gcompl : Term -> Nat × Term
+  | `λt `@  a =>
+    let (n1, t') := gcompl t
+    let (n2, a') := gcompl a
+    (n1 + n2 + 1, t' β[a'])
+  | f `@ a =>
+    let (n1, f') := gcompl f
+    let (n2, a') := gcompl a
+    (n1 + n2, f' `@ a')
+  | `λt =>
+    let (n, t') := gcompl t
+    (n, `λt')
+  | #x => (0, #x)
+
+  theorem gcompl_pcompl : gcompl t = (n, t') -> pcompl t = t' := by
+  intro h; induction t using gcompl.induct generalizing n t'
+  case _ e1 _ _ e2 ih1 ih2 =>
+    simp at *; replace ih1 := ih1 e1
+    replace ih2 := ih2 e2
+    rw [e1, e2] at h; simp at h
+    rw [ih1, ih2]; apply h.2
+  case _ f _ fh _ _ e1 _ _ e2 ih1 ih2 =>
+    cases f
+    case lam => exfalso; apply fh _ rfl
+    all_goals (
+      replace ih1 := ih1 e1
+      replace ih2 := ih2 e2
+      simp; simp at h
+      rw [e2] at h; try rw [e1] at h
+      simp at h
+      rw [ih2]; try rw [ih1]
+      apply h.2
+    )
+  case _ e ih =>
+    simp at *; replace ih := ih e
+    rw [e] at h; simp at h
+    rw [ih]; apply h.2
+  case _ => simp at *; apply h.2
+
+  theorem red_refl : t =β> t := by
+  induction t <;> constructor <;> simp [*]
+
+  theorem red_subst_same σ : s =β> t -> [σ]s =β> [σ]t := by
+  intro h; induction h generalizing σ <;> simp
+  case _ b b' t t' _ _ ih1 ih2 =>
+    have lem : (`λ([^σ]b) `@ ([σ]t)) =β> ([^σ]b') β[[σ]t'] := by
+      apply ParRed.beta (ih1 ^σ) (ih2 _)
+    simp at lem; apply lem
+  case _ ih1 ih2 =>
+    constructor; apply ih1; apply ih2
+  case _ _ ih =>
+    replace ih := ih ^(σ); simp at ih
+    constructor; apply ih
+  case _ => apply red_refl
+
+  theorem red_subst (σ τ : Subst Term) :
+    (∀ n t, σ n = .su t -> ∃ t', τ n = .su t' ∧ t =β> t') ->
+    (∀ n k, σ n = .re k -> τ n = .re k) ->
+    s =β> t -> [σ]s =β> [τ]t
+  := by
+  intro h1 h2 r
+  induction r generalizing σ τ <;> simp
+  case _ b b' t t' _ _ ih1 ih2 =>
+    have lem : (`λ([^σ]b) `@ ([σ]t)) =β> ([^τ]b') β[[τ]t'] := by
+      apply ParRed.beta
+      replace ih1 := ih1 (^σ) (^τ) (Subst.lift_replace red_subst_same h1) (Subst.lift_rename h2)
+      apply ih1; apply ih2 _ _ h1 h2
+    simp at lem; apply lem
+  case _ ih1 ih2 =>
+    apply ParRed.app; apply ih1 _ _ h1 h2; apply ih2 _ _ h1 h2
+  case _ _ ih =>
+    constructor
+    replace ih := ih (^σ) (^τ) (Subst.lift_replace red_subst_same h1) (Subst.lift_rename h2)
+    simp at ih; apply ih
+  case _ x =>
+    generalize udef : σ x = u
+    cases u <;> simp at *
+    case _ y => rw [h2 x y udef]; simp; constructor
+    case _ t =>
+      cases (h1 x t udef); case _ v lem =>
+        rw [lem.1]; simp; apply lem.2
+
+  theorem red_beta : b =β> b' -> t =β> t' -> b β[t] =β> b' β[t'] := by
+  intro r1 r2; apply red_subst
+  case _ =>
+    intro n s h; cases n <;> simp at *
+    case _ => subst h; apply r2
+  case _ =>
+    intro n k h; cases n <;> simp at *; simp [*]
+  case _ => apply r1
+
+  theorem triangle : t =β> s -> s =β> pcompl t := by
+  intro h; induction h <;> simp at * <;> try (constructor <;> simp [*])
+  case _ b b' t t' r1 r2 ih1 ih2 => apply red_beta ih1 ih2
+  case _ a a' f f' _ r2 ih1 ih2 =>
+    cases f <;> simp at * <;> try (constructor <;> simp [*])
+    case _ t =>
+      cases f'
+      case _ => cases ih2
+      case _ => cases r2
+      case _ b =>
+        cases ih2; case _ ih2 =>
+          apply ParRed.beta ih2 ih1
+
+  theorem strip : s =β> t1 -> s =β[n]>* t2 -> ∃ t, t1 =β[n]>* t ∧ t2 =β> t := by
+  intro h1 h2
+  induction h2 generalizing t1
+  case _ t' => exists t1; apply And.intro; apply Star.refl; apply h1
+  case _ n' x y z _r1 r2 ih =>
+    replace ih := ih h1
+    cases ih
+    case _ w ih =>
+      replace r2 := triangle r2
+      have lem := triangle ih.2
+      replace lem := Star.step ih.1 lem
+      exists (pcompl y)
+
+  theorem confluence : s =β[g1]>* t1 -> s =β[g2]>* t2 -> t1 ≡β[g2;g1]≡ t2 := by
+  intro h1 h2
+  induction h1 generalizing t2
+  case _ z =>
+    exists t2; apply And.intro
+    apply h2; apply Star.refl
+  case _ g3 s y t1 _r1 r2 ih =>
+    replace ih := ih h2
+    cases ih; case _ w ih =>
+      have lem := strip r2 ih.1
+      cases lem; case _ q lem =>
+        exists q; apply And.intro
+        apply lem.1; apply Star.step ih.2 lem.2
+
+  theorem refl : t ≡β[g1;g2]≡ t := by
+  exists t; apply And.intro; apply Star.refl; apply Star.refl
+
+  theorem sym : x ≡β[g1;g2]≡ y -> y ≡β[g2;g1]≡ x := by
+  intro h; cases h; case _ w h =>
+    exists w; apply And.intro; apply h.2; apply h.1
+
+  theorem trans : x ≡β[gx;gy1]≡ y -> y ≡β[gy2;gz]≡ z -> x ≡β[gx + gy2;gz + gy1]≡ z := by
+  intro h1 h2
+  cases h1; case _ w1 h1 =>
+  cases h2; case _ w2 h2 =>
+    have lem := confluence h1.2 h2.1
+    cases lem; case _ q lem =>
+      exists q; apply And.intro
+      apply Star.trans h1.1 lem.1
+      apply Star.trans h2.2 lem.2
+
+  theorem pcompl_sound : t =β> (pcompl t) := by apply triangle; apply red_refl
+
+  theorem conv_sound : Conv.conv pcompl g1 g2 a b -> a ≡β[g1;g2]≡ b := by
+  intro h; apply Conv.conv_sound _ h; apply pcompl_sound
+
+end ParRed
+
+namespace Red
+
+  theorem to_par_red : x -β> y -> x =β> y := by
+  intro h; induction h
+  case _ => constructor; apply ParRed.red_refl; apply ParRed.red_refl
+  case _ ih => constructor; apply ih; apply ParRed.red_refl
+  case _ ih => constructor; apply ParRed.red_refl; apply ih
+  case _ ih => constructor; apply ih
+
+  theorem par_sound : x =β[g1;g2]= y -> x ≡β[g1;g2]≡ y := by
+  apply Conv.promote to_par_red
+
+  -- theorem from_gcompl : ParRed.gcompl t = (n, t') -> x -β[n]>* y := by sorry
+
+end Red
+
+namespace SpineRed
+
+  theorem to_par_red : x -s> y -> x =β> y := by
+  intro h; induction h
+  case _ => constructor; apply ParRed.red_refl; apply ParRed.red_refl
+  case _ ih1 ih2 => constructor; apply ih2; apply ih1
+  case _ ih => constructor; apply ih
+
+  theorem par_sound : x =s[g1;g2]= y -> x ≡β[g1;g2]≡ y := by
+  apply Conv.promote to_par_red
+
+end SpineRed
