Untyped/Subst.lean
@@ -1,5 +1,4 @@
 
-
 def Ren : Type := Nat -> Nat
 
 namespace Subst
@@ -22,7 +21,9 @@ def seq_cons : T -> (Nat -> T) -> (Nat -> T)
 infix:70 "::" => seq_cons
 
 section
-  variable {T : Type} [SubstitutionType T]
+  variable
+    {F : Type -> Type}
+    {T : Type} [SubstitutionType T]
 
   open SubstitutionType
 
@@ -50,7 +51,7 @@ section
       | .su t => .su (Ren.apply (λ n => n + 1) t)
       | .re k => .re (k + 1)
 
-    def apply : Subst T -> T -> T := smap lift
+    def apply (σ : Subst T) : T -> T := smap lift σ
 
     def compose : Subst T -> Subst T -> Subst T
     | σ, τ, n => match (σ n) with
@@ -61,6 +62,14 @@ section
 
   def I : Subst T := λ n => .re n
   def S : Subst T := λ n => .re (n + 1)
+
+  omit [SubstitutionType T] in
+  @[simp]
+  theorem I_action : @I T n = .re n := by unfold I; simp
+
+  omit [SubstitutionType T] in
+  @[simp]
+  theorem S_action : @S T n = .re (n + 1) := by unfold S; simp
 
   prefix:max "^" => Subst.lift
   notation:90 "[" σ "]" t:89 => Subst.apply σ t
@@ -73,7 +82,7 @@ section
   class SubstitutionTypeLaws (T : Type) [SubstitutionType T] where
     apply_id {t : T} : [I]t = t
     apply_compose {s : T} {σ τ : Subst T} : [τ][σ]s = [τ ⊙ σ]s
-    apply_stable {σ : Subst T} : r.to = σ -> Ren.apply r = Subst.apply σ
+    apply_stable {σ : Subst T} : r.to = σ -> Ren.apply r = Subst.apply  σ
 end
 
 namespace Subst
@@ -98,7 +107,7 @@ section
       unfold Ren.to; unfold Ren.lift; simp
       unfold Subst.lift; simp
     case _ n =>
-      generalize lhsdef : (r.lift.to) (n + 1) = lhs
+      generalize lhsdef : ((@Ren.to T r.lift)) (n + 1) = lhs
       generalize rhsdef : (^(@Ren.to T r)) (n + 1) = rhs
       unfold Ren.to at lhsdef; simp at *
       unfold Ren.lift at lhsdef; simp at *
@@ -115,7 +124,7 @@ section
 
   omit [SubstitutionTypeLaws T] in
   @[simp]
-  theorem valid1 {s t : T} : s β[t] = [.su t :: I]s := by simp
+  theorem valid1 {s : T} : s β[t] = [.su t :: I]s := by simp
 
   @[simp] -- ⇑σ = 0.(σ ◦ S)
   theorem valid3 {σ : Subst T} : ^σ = .re 0 :: (S ⊙ σ) := by
@@ -189,98 +198,131 @@ section
     case _ => simp
     case _ => simp; unfold S; unfold Subst.compose; simp
 
+  theorem lift_rename {σ τ : Subst T} :
+    (∀ n k, σ n = .re k -> τ n = .re k) ->
+    ∀ n k, ^σ n = .re k -> ^τ n = .re k
+  := by
+  intro h1 n k h2
+  cases n <;> simp at *
+  case _ => exact h2
+  case _ n =>
+    unfold Subst.compose at *; simp at *
+    generalize ydef : σ n = y at *
+    cases y <;> simp at *
+    case _ i => rw [h1 n i ydef]; simp [*]
+
+  theorem lift_replace
+    {R : T -> T -> Prop}
+    (Rs : ∀ {t t' : T} σ, R t t' -> R ([σ]t) ([σ]t'))
+    {σ τ : Subst T}
+  :
+    (∀ n t, σ n = .su t -> ∃ t', τ n = .su t' ∧ R t t') ->
+    ∀ n t, ^σ n = .su t -> ∃ t', ^τ n = .su t' ∧ R t t'
+  := by
+  intro h1 n t h2
+  cases n <;> simp at *
+  case _ n =>
+    unfold Subst.compose at h2; simp at h2
+    generalize udef : σ n = u at *
+    cases u <;> simp at *
+    case _ s =>
+      replace h1 := h1 n s udef
+      unfold Subst.compose; simp
+      generalize vdef : τ n = v at *
+      cases v <;> simp at *
+      case _ w => rw [<-h2]; apply Rs S h1
+
 end
 
-  macro "solve_compose" Term:term "," apply_stable:term "," s:term "," σ:term "," τ:term : tactic => `(tactic| {
-      have lem1 (τ : Subst $Term) : ^τ ⊙ (Ren.to (λ x => x + 1)) = (Ren.to (λ x => x + 1)) ⊙ τ := by
-        funext; unfold Subst.compose; simp; unfold Ren.to; simp; case _ x =>
-          generalize zdef : τ x = z; generalize vdef : ^τ (x + 1) = v
-          unfold Subst.lift at vdef; simp at vdef; rw [zdef] at vdef
-          cases z
-          case _ => simp at *; simp [*]
-          case _ =>
-            simp at *; rw [<-vdef]; simp;
-            rw [@$apply_stable (λ x => x + 1) (λ x => .re (x + 1)) (by unfold Ren.to; simp)]
-      have lem2 (σ : Subst $Term) (e : Ren) : ^(σ ⊙ (e.to)) = ^σ ⊙ ^(e.to) := by
-        funext; case _ n =>
-        cases n
-        . unfold Ren.to; unfold Subst.compose; unfold Subst.lift; simp
-        case _ n =>
-          generalize lhsdef : (^σ ⊙ ^(e.to)) (n + 1) = lhs
-          unfold Subst.lift; simp
-          unfold Subst.compose; unfold Ren.to; simp
-          subst lhs; unfold Subst.compose; unfold Subst.lift; simp
-          unfold Ren.to; simp
-      have lem3 {σ : Subst $Term} {e : Ren} s : [σ][e.to]s = [σ ⊙ (e.to)]s := by
-        induction s generalizing σ e
-        any_goals simp [*]
-        any_goals (rw [<-Subst.lift_lemma]; simp [*])
-        any_goals (
-          unfold Subst.compose; simp
-          unfold Subst.apply; simp; split <;> simp at *
-          unfold Ren.to; simp [*]
-          unfold Ren.to; simp [*]
-        )
-      have lem4 (σ τ : Subst $Term) : σ ⊙ τ ⊙ (Ren.to (λ x => x + 1)) = σ ⊙ (τ ⊙ (Ren.to (λ x => x + 1))) := by
-        funext; case _ x =>
-        cases x; any_goals (unfold Subst.compose; unfold Ren.to; simp)
-      have lem5 (r1 r2 : Ren) (τ : Subst $Term) : r1.to ⊙ (r2.to ⊙ τ) = r1.to ⊙ r2.to ⊙ τ := by
-        funext; case _ x =>
-          unfold Subst.compose; simp
-          cases τ x <;> simp at *
-          case _ t =>
-            have lem : [fun x => Subst.Action.re (r1 (r2 x))]t = [r1.to ⊙ r2.to]t := by
-              unfold Subst.compose; unfold Ren.to; simp
-            rw [<-lem3] at lem; unfold Ren.to at lem; simp at lem
-            unfold Ren.to; simp; rw [lem]
-      have lem6 (e : Ren) (τ : Subst $Term) : ^(e.to) ⊙ ^τ = ^((e.to) ⊙ τ) := by
-        funext; case _ n =>
-        cases n
-        . unfold Subst.compose; unfold Subst.lift; simp
-        case _ n =>
-          have lem : ((^(e.to) ⊙ ^τ) ⊙ (Ren.to (fun x => x + 1))) n = (^(e.to ⊙ τ) ⊙ (Ren.to (fun x => x + 1))) n := by {
-            rw [lem1, lem4, lem1]
-            rw [<-Subst.lift_lemma, lem5]; simp
-            rw [Subst.lift_lemma, lem1, lem5]
-          }
-          unfold Subst.compose at lem; unfold Ren.to at lem
-          unfold Subst.compose; unfold Ren.to
-          simp at lem; simp [*]
-      have lem7 (τ : Subst $Term) (e : Ren) s : [e.to][τ]s = [(e.to) ⊙ τ]s := by
-        induction s generalizing τ e
-        any_goals simp [*]
-        any_goals (rw [<-lem6, <-Subst.lift_lemma]; simp [*])
-        any_goals (
-          unfold Subst.compose; simp
-          unfold Subst.apply; simp; split <;> simp [*]
-        )
-      have lem8 (σ τ : Subst $Term) : σ ⊙ ((Ren.to (λ x => x + 1)) ⊙ τ) = σ ⊙ (Ren.to (λ x => x + 1)) ⊙ τ := by
-        funext; case _ x =>
-          unfold Subst.compose; simp
-          cases τ x <;> simp at *
-          rw [lem3]; unfold Subst.compose; simp
-      have lem9 (σ τ : Subst $Term) : (Ren.to (λ x => x + 1)) ⊙ (σ ⊙ τ) = (Ren.to (λ x => x + 1)) ⊙ σ ⊙ τ := by
-        funext; case _ x =>
-          unfold Subst.compose; simp
-          cases τ x <;> simp at *
-          rw [lem7]; unfold Subst.compose; simp
-      have lem10 (σ τ : Subst $Term) : ^σ ⊙ ^τ = ^(σ ⊙ τ) := by
-        funext; case _ x =>
-        cases x
-        case _ => unfold Subst.compose; unfold Subst.lift; simp
-        case _ n =>
-          have lem : ((^σ ⊙ ^τ) ⊙ (Ren.to (λ x => x + 1))) n
-            = (^(σ ⊙ τ) ⊙ (Ren.to (λ x => x + 1))) n
-          := by rw [lem1, lem4, lem1, lem8, lem1, lem9]
-          unfold Subst.compose at lem; unfold Ren.to at lem
-          unfold Subst.compose
-          simp at lem; simp [*]
-      induction $s generalizing $τ $σ
-      all_goals (simp at *; try simp [*])
-      all_goals (
+  macro "solve_compose" Ty:term "," apply_stable:term "," s:term "," σ:term "," τ:term : tactic => `(tactic| {
+    have lem1 (τ : Subst $Ty) : ^τ ⊙ (Ren.to (λ x => x + 1)) = (Ren.to (λ x => x + 1)) ⊙ τ := by
+      funext; unfold Subst.compose; simp; unfold Ren.to; simp; case _ x =>
+        generalize zdef : τ x = z; generalize vdef : ^τ (x + 1) = v
+        unfold Subst.lift at vdef; simp at vdef; rw [zdef] at vdef
+        cases z
+        case _ => simp at *; simp [*]
+        case _ =>
+          simp at *; rw [<-vdef]; simp;
+          rw [@$apply_stable (λ x => x + 1) (λ x => .re (x + 1)) (by unfold Ren.to; simp)]
+    have lem2 (σ : Subst $Ty) (e : Ren) : ^(σ ⊙ (e.to)) = ^σ ⊙ ^(e.to) := by
+      funext; case _ n =>
+      cases n
+      . unfold Ren.to; unfold Subst.compose; unfold Subst.lift; simp
+      case _ n =>
+        generalize lhsdef : (^σ ⊙ ^(e.to)) (n + 1) = lhs
+        unfold Subst.lift; simp
+        unfold Subst.compose; unfold Ren.to; simp
+        subst lhs; unfold Subst.compose; unfold Subst.lift; simp
+        unfold Ren.to; simp
+    have lem3 {σ : Subst $Ty} {e : Ren} s : [σ][e.to]s = [σ ⊙ (e.to)]s := by
+      induction s generalizing σ e
+      any_goals simp [*]
+      any_goals (rw [<-Subst.lift_lemma]; simp [*])
+      any_goals (
+        unfold Subst.compose; simp
+        unfold Subst.apply; simp; split <;> simp at *
+      )
+      any_goals (unfold Ren.to; simp [*])
+    have lem4 (σ τ : Subst $Ty) : σ ⊙ τ ⊙ (Ren.to (λ x => x + 1)) = σ ⊙ (τ ⊙ (Ren.to (λ x => x + 1))) := by
+      funext; case _ x =>
+      cases x; any_goals (unfold Subst.compose; unfold Ren.to; simp)
+    have lem5 (r1 r2 : Ren) (τ : Subst $Ty) : r1.to ⊙ (r2.to ⊙ τ) = r1.to ⊙ r2.to ⊙ τ := by
+      funext; case _ x =>
+        unfold Subst.compose; simp
+        cases τ x <;> simp at *
+        case _ t =>
+          have lem : [fun x => Subst.Action.re (r1 (r2 x))]t = [r1.to ⊙ r2.to]t := by
+            unfold Subst.compose; unfold Ren.to; simp
+          rw [<-lem3] at lem; unfold Ren.to at lem; simp at lem
+          unfold Ren.to; simp; rw [lem]
+    have lem6 (e : Ren) (τ : Subst $Ty) : ^(e.to) ⊙ ^τ = ^((e.to) ⊙ τ) := by
+      funext; case _ n =>
+      cases n
+      . unfold Subst.compose; unfold Subst.lift; simp
+      case _ n =>
+        have lem : ((^(e.to) ⊙ ^τ) ⊙ (Ren.to (fun x => x + 1))) n = (^(e.to ⊙ τ) ⊙ (Ren.to (fun x => x + 1))) n := by {
+          rw [lem1, lem4, lem1]
+          rw [<-Subst.lift_lemma, lem5]; simp
+          rw [Subst.lift_lemma, lem1, lem5]
+        }
+        unfold Subst.compose at lem; unfold Ren.to at lem
+        unfold Subst.compose; unfold Ren.to
+        simp at lem; simp [*]
+    have lem7 (τ : Subst $Ty) (e : Ren) s : [e.to][τ]s = [(e.to) ⊙ τ]s := by
+      induction s generalizing τ e
+      any_goals simp [*]
+      any_goals (rw [<-lem6, <-Subst.lift_lemma]; simp [*])
+      any_goals (
         unfold Subst.compose; simp
         unfold Subst.apply; simp; split <;> simp [*]
       )
+    have lem8 (σ τ : Subst $Ty) : σ ⊙ ((Ren.to (λ x => x + 1)) ⊙ τ) = σ ⊙ (Ren.to (λ x => x + 1)) ⊙ τ := by
+      funext; case _ x =>
+        unfold Subst.compose; simp
+        cases τ x <;> simp at *
+        rw [lem3]; unfold Subst.compose; simp
+    have lem9 (σ τ : Subst $Ty) : (Ren.to (λ x => x + 1)) ⊙ (σ ⊙ τ) = (Ren.to (λ x => x + 1)) ⊙ σ ⊙ τ := by
+      funext; case _ x =>
+        unfold Subst.compose; simp
+        cases τ x <;> simp at *
+        rw [lem7]; unfold Subst.compose; simp
+    have lem10 (σ τ : Subst $Ty) : ^σ ⊙ ^τ = ^(σ ⊙ τ) := by
+      funext; case _ x =>
+      cases x
+      case _ => unfold Subst.compose; unfold Subst.lift; simp
+      case _ n =>
+        have lem : ((^σ ⊙ ^τ) ⊙ (Ren.to (λ x => x + 1))) n
+          = (^(σ ⊙ τ) ⊙ (Ren.to (λ x => x + 1))) n
+        := by rw [lem1, lem4, lem1, lem8, lem1, lem9]
+        unfold Subst.compose at lem; unfold Ren.to at lem
+        unfold Subst.compose
+        simp at lem; simp [*]
+    induction $s generalizing $τ $σ
+    all_goals (simp at *; try simp [*])
+    all_goals (
+      unfold Subst.compose; simp
+      unfold Subst.apply; simp; split <;> simp [*]
+    )
   })
 
 end Subst
