Fomega/Everything.lean
@@ -1,5 +1,4 @@
 
-import Fomega.Ctx
 import Fomega.Proof
 import Fomega.PreProof
 import Fomega.Basic
