Untyped/Value.lean
@@ -1,82 +1,82 @@
-import Untyped.Subst
+-- import Untyped.Subst
 
-inductive ValueVariant : Type where
-| term | spine
+-- inductive ValueVariant : Type where
+-- | term | spine
 
-inductive Value : ValueVariant -> Type where
-| nil : Value .spine
-| cons : Value .term -> Value .spine -> Value .spine
-| var : Nat -> Value .spine -> Value .term
-| lam : Value .term -> Value .spine -> Value .term
-deriving Repr
+-- inductive Value : ValueVariant -> Type where
+-- | nil : Value .spine
+-- | cons : Value .term -> Value .spine -> Value .spine
+-- | var : Nat -> Value .spine -> Value .term
+-- | lam : Value .term -> Value .spine -> Value .term
+-- deriving Repr
 
-namespace Value
-  @[simp]
-  def concat : Value .spine -> Value .spine -> Value .spine
-  | .nil, sp => sp
-  | .cons hd tl, sp => .cons hd (concat tl sp)
+-- namespace Value
+--   @[simp]
+--   def concat : Value .spine -> Value .spine -> Value .spine
+--   | .nil, sp => sp
+--   | .cons hd tl, sp => .cons hd (concat tl sp)
 
-  @[simp]
-  def add_spine : Value .term -> Value .spine -> Value .term
-  | .var x s1, s2 => .var x (concat s1 s2)
-  | .lam t s1, s2 => .lam t (concat s1 s2)
+--   @[simp]
+--   def add_spine : Value .term -> Value .spine -> Value .term
+--   | .var x s1, s2 => .var x (concat s1 s2)
+--   | .lam t s1, s2 => .lam t (concat s1 s2)
 
-  @[simp]
-  def smap (lf : Subst.Lift (∀ {v}, Value v)) (f : Nat -> Subst.Action (∀ {v}, Value v)) : ∀ {v}, Value v -> Value v
-  | _, nil => sorry
-  | _, cons hd tl => sorry
-  | _, var x sp =>
-    let sp := smap lf f sp
-    match f x with
-    | .re y => var y sp
-    | .su t => t.add_spine sp
-  | _, lam t sp => lam (smap lf (lf f) t) (smap lf f sp)
-end Value
+--   @[simp]
+--   def smap (lf : Subst.Lift (∀ {v}, Value v)) (f : Nat -> Subst.Action (∀ {v}, Value v)) : ∀ {v}, Value v -> Value v
+--   | _, nil => sorry
+--   | _, cons hd tl => sorry
+--   | _, var x sp =>
+--     let sp := smap lf f sp
+--     match f x with
+--     | .re y => var y sp
+--     | .su t => t.add_spine sp
+--   | _, lam t sp => lam (smap lf (lf f) t) (smap lf f sp)
+-- end Value
 
-@[simp]
-instance substType_Value : SubstitutionType Value where
-  smap := Value.smap
+-- @[simp]
+-- instance substType_Value : SubstitutionType Value where
+--   smap := Value.smap
 
-namespace Value
+-- namespace Value
 
-  @[simp] -- 0[s.σ ] = s
-  theorem subst_var_replace
-    : [.su s :: σ]var 0 sp = s.add_spine sp
-  := by sorry
+--   @[simp] -- 0[s.σ ] = s
+--   theorem subst_var_replace
+--     : [.su s :: σ]var 0 sp = s.add_spine sp
+--   := by sorry
 
-  @[simp] -- 0[s.σ ] = s
-  theorem subst_var_rename
-    : [.re k :: σ]var 0 sp = var k (List.map (Subst.apply (.re k :: σ)) sp)
-  := by sorry
+--   @[simp] -- 0[s.σ ] = s
+--   theorem subst_var_rename
+--     : [.re k :: σ]var 0 sp = var k (List.map (Subst.apply (.re k :: σ)) sp)
+--   := by sorry
 
-  @[simp]
-  theorem subst_lam : [σ](lam t sp) = lam ([^σ]t) (List.map (Subst.apply σ) sp)  := by sorry
+--   @[simp]
+--   theorem subst_lam : [σ](lam t sp) = lam ([^σ]t) (List.map (Subst.apply σ) sp)  := by sorry
 
-  theorem apply_id {t : Value} : [I]t = t := by
-  have lem : ^I = @I Value := by
-    funext; case _ x =>
-    cases x; all_goals (unfold Subst.lift; unfold I; simp)
-  induction t
-  all_goals (simp at * <;> try simp [*])
-  unfold Subst.apply; unfold I; simp
+--   theorem apply_id {t : Value} : [I]t = t := by
+--   have lem : ^I = @I Value := by
+--     funext; case _ x =>
+--     cases x; all_goals (unfold Subst.lift; unfold I; simp)
+--   induction t
+--   all_goals (simp at * <;> try simp [*])
+--   unfold Subst.apply; unfold I; simp
 
-  theorem apply_stable {r : Ren} {σ : Subst Value} : r.to = σ -> r.apply = σ.apply := by sorry
-  -- intro h; funext; case _ x =>
-  --   unfold Ren.apply; simp at *
-  --   unfold Ren.to; simp
-  --   induction x generalizing r σ <;> simp at *
-  --   case _ x => unfold Subst.apply; simp; rw [<-h]; unfold Ren.to; simp
-  --   case _ => simp [*]
-  --   case _ =>
-  --     simp [*]; rw [Subst.lift_lemma, <-h]
-  --     unfold Ren.fro; simp
+--   theorem apply_stable {r : Ren} {σ : Subst Value} : r.to = σ -> r.apply = σ.apply := by sorry
+--   -- intro h; funext; case _ x =>
+--   --   unfold Ren.apply; simp at *
+--   --   unfold Ren.to; simp
+--   --   induction x generalizing r σ <;> simp at *
+--   --   case _ x => unfold Subst.apply; simp; rw [<-h]; unfold Ren.to; simp
+--   --   case _ => simp [*]
+--   --   case _ =>
+--   --     simp [*]; rw [Subst.lift_lemma, <-h]
+--   --     unfold Ren.fro; simp
 
-  theorem apply_compose {s : Value} {σ τ : Subst Value} : [τ][σ]s = [τ ⊙ σ]s := by
-    solve_compose Value, apply_stable, s, σ, τ
+--   theorem apply_compose {s : Value} {σ τ : Subst Value} : [τ][σ]s = [τ ⊙ σ]s := by
+--     solve_compose Value, apply_stable, s, σ, τ
 
-end Value
+-- end Value
 
-instance substTypeLaws_Value : SubstitutionTypeLaws Value where
-  apply_id := Value.apply_id
-  apply_compose := Value.apply_compose
-  apply_stable := Value.apply_stable
+-- instance substTypeLaws_Value : SubstitutionTypeLaws Value where
+--   apply_id := Value.apply_id
+--   apply_compose := Value.apply_compose
+--   apply_stable := Value.apply_stable
